coq/proof/SoundBase.v
@@ -15,12 +15,67 @@ Require Import paco.
 Import Opsem.
 
 Require Import TODO.
+Require Import Decs.
 Require Import Validator.
 Require Import GenericValues.
 Require Import SimulationLocal.
 Require Import Inject.
 Require InvMem.
 Require InvState.
+
+Set Implicit Arguments.
+
+
+Ltac simtac0 :=
+  try match goal with
+      | [H: ?a = ?a |- _] => clear H
+      | [H: is_true true |- _] => clear H
+      | [H: Some _ = Some _ |- _] => inv H
+      | [H: context[let (_, _) := ?p in _] |- _] => destruct p
+      | [H: negb _ = true |- _] =>
+        apply negb_true_iff in H
+      | [H: negb _ = false |- _] =>
+        apply negb_false_iff in H
+      | [H: andb _ _ = true |- _] => apply andb_true_iff in H; destruct H
+
+      | [H: proj_sumbool (id_dec ?a ?b) = true |- _] =>
+        destruct (id_dec a b)
+      | [H: proj_sumbool (typ_dec ?a ?b) = true |- _] =>
+        destruct (typ_dec a b)
+      | [H: proj_sumbool (l_dec ?a ?b) = true |- _] =>
+        destruct (l_dec a b)
+      | [H: proj_sumbool (fheader_dec ?a ?b) = true |- _] =>
+        destruct (fheader_dec a b)
+      | [H: proj_sumbool (noret_dec ?a ?b) = true |- _] =>
+        destruct (noret_dec a b)
+      | [H: proj_sumbool (clattrs_dec ?a ?b) = true |- _] =>
+        destruct (clattrs_dec a b)
+      | [H: proj_sumbool (varg_dec ?a ?b) = true |- _] =>
+        destruct (varg_dec a b)
+      | [H: proj_sumbool (layouts_dec ?a ?b) = true |- _] => destruct (layouts_dec a b)
+      | [H: proj_sumbool (namedts_dec ?a ?b) = true |- _] => destruct (namedts_dec a b)
+      | [H: productInModuleB_dec ?a ?b = left _ |- _] => destruct (productInModuleB_dec a b)
+
+      | [H: context[match ?c with
+                    | [] => _
+                    | _::_ => _
+                    end] |- _] =>
+        let COND := fresh "COND" in
+        destruct c eqn:COND
+      | [H: context[match ?c with
+                    | Some _ => _
+                    | None => _
+                    end] |- _] =>
+        let COND := fresh "COND" in
+        destruct c eqn:COND
+      | [H: context[if ?c then _ else _] |- _] =>
+        let COND := fresh "COND" in
+        destruct c eqn:COND
+      end;
+  unfold Debug.debug_print_validation_process, Debug.debug_print in *;
+  try subst; ss.
+
+Ltac simtac := repeat simtac0.
 
 (* TODO: m_src, m_tgt, conf_src, conf_tgt *)
 Inductive valid_conf
@@ -41,3 +96,15 @@ Lemma lookupBlockViaLabelFromFdef_spec
   lookupBlockViaLabelFromFdef fdef l =
   lookupAL _ fdef.(get_blocks) l.
 Proof. destruct fdef. ss. Qed.
+
+(* TODO: position *)
+Definition ite A (c:bool) (a b:A): A :=
+  if c then a else b.
+
+(* TODO: position *)
+Lemma ite_spec A c (a b:A):
+  ite c a b = if c then a else b.
+Proof. ss. Qed.
+
+(* TODO: position *)
+Opaque ite.
