coq/proof/SimulationLocal.v
@@ -89,8 +89,6 @@ Section SimLocal.
       st2_src
       id2_src noret2_src clattrs2_src typ2_src varg2_src fun2_src params2_src cmds2_src
       id1_tgt noret1_tgt clattrs1_tgt typ1_tgt varg1_tgt fun1_tgt params1_tgt cmds1_tgt
-      funval2_src args2_src
-      funval1_tgt args1_tgt
       (STEP: sop_star conf_src st1_src st2_src E0)
       (CMDS_SRC: st2_src.(EC).(CurCmds) = (insn_call id2_src noret2_src clattrs2_src typ2_src varg2_src fun2_src params2_src)::cmds2_src)
       (CMDS_TGT: st1_tgt.(EC).(CurCmds) = (insn_call id1_tgt noret1_tgt clattrs1_tgt typ1_tgt varg1_tgt fun1_tgt params1_tgt)::cmds1_tgt)
@@ -98,30 +96,37 @@ Section SimLocal.
       (CLATTRS: clattrs2_src = clattrs1_tgt)
       (TYP: typ2_src = typ1_tgt)
       (VARG: varg2_src = varg1_tgt)
-      (FUN_SRC: getOperandValue conf_src.(CurTargetData) fun2_src st2_src.(EC).(Locals) conf_src.(Globals) = Some funval2_src)
-      (FUN_TGT: getOperandValue conf_tgt.(CurTargetData) fun1_tgt st1_tgt.(EC).(Locals) conf_tgt.(Globals) = Some funval1_tgt)
-      (FUNVAL: genericvalues_inject.gv_inject inv1.(InvMem.Rel.inject) funval2_src funval1_tgt)
-      (PARAMS_SRC: params2GVs conf_src.(CurTargetData) params2_src st2_src.(EC).(Locals) conf_src.(Globals) = Some args2_src)
-      (PARAMS_TGT: params2GVs conf_tgt.(CurTargetData) params1_tgt st1_tgt.(EC).(Locals) conf_tgt.(Globals) = Some args1_tgt)
-      (ARGS: list_forall2 (genericvalues_inject.gv_inject inv1.(InvMem.Rel.inject)) args2_src args1_tgt)
+      (FUN:
+         forall funval2_src
+           (FUN_SRC: getOperandValue conf_src.(CurTargetData) fun2_src st2_src.(EC).(Locals) conf_src.(Globals) = Some funval2_src),
+         exists funval1_tgt,
+           <<FUN_TGT: getOperandValue conf_tgt.(CurTargetData) fun1_tgt st1_tgt.(EC).(Locals) conf_tgt.(Globals) = Some funval1_tgt>> /\
+           <<INJECT: genericvalues_inject.gv_inject inv1.(InvMem.Rel.inject) funval2_src funval1_tgt>>)
+      (ARGS:
+         forall args2_src
+           (ARGS_SRC: params2GVs conf_src.(CurTargetData) params2_src st2_src.(EC).(Locals) conf_src.(Globals) = Some args2_src),
+         exists args1_tgt,
+           <<ARGS_TGT: params2GVs conf_tgt.(CurTargetData) params1_tgt st1_tgt.(EC).(Locals) conf_tgt.(Globals) = Some args1_tgt>> /\
+           <<INJECT: list_forall2 (genericvalues_inject.gv_inject inv1.(InvMem.Rel.inject)) args2_src args1_tgt>>)
       (MEM: InvMem.Rel.sem conf_src conf_tgt st2_src.(Mem) st1_tgt.(Mem) inv1)
       (RETURN:
          forall inv3 mem3_src mem3_tgt retval3_src retval3_tgt
            (INCR: InvMem.Rel.le inv1 inv3)
            (MEM: InvMem.Rel.sem conf_src conf_tgt mem3_src mem3_tgt inv3)
-           (RET: noret2_src = false)
            (RETVAL: genericvalues_inject.gv_inject inv3.(InvMem.Rel.inject) retval3_src retval3_tgt),
-         exists idx3,
-           sim_local
-             stack0_src stack0_tgt inv3 idx3
-             (mkState
-                (mkEC st2_src.(EC).(CurFunction) st2_src.(EC).(CurBB) cmds2_src st2_src.(EC).(Terminator) st2_src.(EC).(Locals) st2_src.(EC).(Allocas))
-                st2_src.(ECS)
-                mem3_src)
-             (mkState
-                (mkEC st1_tgt.(EC).(CurFunction) st1_tgt.(EC).(CurBB) cmds1_tgt st1_tgt.(EC).(Terminator) st1_tgt.(EC).(Locals) st1_tgt.(EC).(Allocas))
-                st1_tgt.(ECS)
-                mem3_tgt))
+         exists idx4 inv4,
+           <<MEMLE: InvMem.Rel.le inv3 inv4>> /\
+           <<SIM:
+             sim_local
+               stack0_src stack0_tgt inv4 idx4
+               (mkState
+                  (mkEC st2_src.(EC).(CurFunction) st2_src.(EC).(CurBB) cmds2_src st2_src.(EC).(Terminator) st2_src.(EC).(Locals) st2_src.(EC).(Allocas))
+                  st2_src.(ECS)
+                  mem3_src)
+               (mkState
+                  (mkEC st1_tgt.(EC).(CurFunction) st1_tgt.(EC).(CurBB) cmds1_tgt st1_tgt.(EC).(Terminator) st1_tgt.(EC).(Locals) st1_tgt.(EC).(Allocas))
+                  st1_tgt.(ECS)
+                  mem3_tgt)>>)
 
   | _sim_local_step
       (PROGRESS: ~ stuck_state conf_tgt st1_tgt)
@@ -129,10 +134,10 @@ Section SimLocal.
          forall st3_tgt event
            (STEP: sInsn conf_tgt st1_tgt st3_tgt event),
          exists st2_src st3_src st3_tgt inv3 idx3,
-           sop_star conf_src st1_src st2_src E0 /\
-           sInsn_indexed conf_src st2_src st3_src idx1 idx3 event /\
-           InvMem.Rel.le inv1 inv3 /\
-           sim_local stack0_src stack0_tgt inv3 idx3 st3_src st3_tgt)
+           <<TAU: sop_star conf_src st1_src st2_src E0>> /\
+           <<EVT: sInsn_indexed conf_src st2_src st3_src idx1 idx3 event>> /\
+           <<MEMLE: InvMem.Rel.le inv1 inv3>> /\
+           <<SIM: sim_local stack0_src stack0_tgt inv3 idx3 st3_src st3_tgt>>)
   .
   Hint Constructors _sim_local.
 
